src/Solver/Solvers.dfy
@@ -1,18 +1,220 @@
 module Solvers {
+  import Smt
+  import Z3SmtSolver // TODO: Use solver factories?
   export
-    provides Solver, Solver.Extend, Solver.Prove, Solver.Record
+    provides Solver, Solver.Extend, Solver.Prove, Solver.Record, Solver.Empty
+    reveals SolverState
+    reveals Context
+    provides SolverState.solver, SolverState.Valid, SolverState.assumptions
+    provides SolverState.ValidFor
+    provides Smt
+    provides B
     provides SolverExpr
 
   import opened SolverExpr
+  import B = Basics
+
+  datatype ProofResult =
+      Proved
+    | Unproved(reason: string)
+  
+  datatype Context =
+    | Assumption(assumed: SExpr)
+    | Declaration(name: string, inputType: SExpr, outputType: SExpr)
+  {
+    function ToSmt(): Smt.Context {
+      match this {
+        case Assumption(assumed) =>
+          Smt.Assumption(assumed.ToString())
+        case Declaration(name, inputType, outputTpe) =>
+          Smt.Declaration(name, inputType.ToString(), outputType.ToString())
+      }
+    }
+    function ToString(): string {
+      ToSmt().ToString()
+    }
+  }
+
+  // This solver state can backtrack, however, it cannot spawn new Z3 instances
+  class SolverState {
+    ghost var assumptions: B.List<Context>
+    ghost var assumptionsStacks: B.List<B.List<Context>>
+
+    const solver: Smt.Solver
+
+    constructor(solver: Smt.Solver)
+    // Should be a fresh solver
+      requires solver.CommandStacks() == B.Cons(B.Nil, B.Nil)
+      requires solver.Valid()
+      ensures solver == this.solver
+      ensures this.Valid()
+      ensures this.ValidFor(Solver.Empty())
+    {
+      this.solver := solver;
+      this.assumptions := B.Nil;
+      this.assumptionsStacks := B.Cons(B.Nil, B.Nil);
+    }
+
+    ghost predicate ValidFor(s: Solver) reads this {
+      s.assumptions == this.assumptions.ToReverseSeq()
+    }
+    
+    static ghost predicate assumptionsSyncCommands(
+      assumptionsStacks: B.List<B.List<Context>>,
+      commandStacks: B.List<B.List<string>>
+    ) {
+      || (assumptionsStacks.Nil? && commandStacks.Nil?)
+      || (assumptionsStacks.Cons? && commandStacks.Cons?
+        && commandStacks.head == assumptionsStacks.head.Map((a: Context) => a.ToSmt().ToString())
+        && assumptionsSyncCommands(assumptionsStacks.tail, commandStacks.tail)
+      )
+    }
+
+    ghost predicate Valid() reads this, solver, solver.process
+    {
+      solver.Valid()
+      && this as object !in {solver, solver.process}
+      && B.ListFlatten(assumptionsStacks) == assumptions
+      && assumptionsSyncCommands(assumptionsStacks, solver.CommandStacks())
+    }
+
+    ghost predicate ValidBeforePop() reads this, solver, solver.process
+    {
+      solver.Valid()
+      && this as object !in {solver, solver.process}
+      && B.ListFlatten(assumptionsStacks) == assumptions
+      && assumptionsStacks.Cons?
+      && assumptionsSyncCommands(assumptionsStacks.tail, solver.CommandStacks().tail)
+    }
+
+    method Push()
+      requires Valid()
+      modifies this, solver, solver.process
+      ensures Valid()
+      ensures assumptions == old(assumptions)
+      ensures assumptionsStacks.tail == old(assumptionsStacks)
+    {
+      solver.Push();
+      assumptionsStacks := B.Cons(B.Nil, assumptionsStacks);
+    }
+
+    method Pop()
+      requires ValidBeforePop()
+      requires solver.CommandStacks().DoubleCons?
+      modifies solver, solver.process
+      modifies this
+      ensures Valid()
+      ensures assumptionsStacks == old(this.assumptionsStacks.tail)
+    {
+      solver.Pop();
+      assumptions := assumptions.DropAsMuchAsHeadOf(assumptionsStacks);
+      assumptionsStacks := assumptionsStacks.tail;
+    }
+
+    method AddContext(context: Context)
+      requires Valid()
+      modifies this, solver, solver.process
+      ensures Valid()
+      ensures assumptions == B.Cons(context, old(assumptions))
+      ensures assumptionsStacks.head.Cons?
+      ensures assumptionsStacks == old(assumptionsStacks.(
+        head := B.Cons(context, assumptionsStacks.head)))
+    {
+      match context {
+        case Declaration(name, inputTpe, outputTpe) =>
+          solver.DeclareFun(name, inputTpe.ToString(), outputTpe.ToString());
+        case Assumption(e) =>
+          solver.Assume(e.ToString());
+      }
+      assumptions := B.Cons(context, assumptions);
+      assumptionsStacks := assumptionsStacks.(
+        head := B.Cons(context, assumptionsStacks.head));
+    }
+
+    method DeclareSymbol(name: string, inputTpe: SExpr, outputTpe: SExpr)
+      requires Valid()
+      modifies this, solver, solver.process
+      ensures Valid()
+      ensures assumptions == B.Cons(Declaration(name, inputTpe, outputTpe), old(assumptions))
+      ensures assumptionsStacks.head.Cons?
+      ensures assumptionsStacks == old(assumptionsStacks.(
+        head := B.Cons(Declaration(name, inputTpe, outputTpe), assumptionsStacks.head)))
+    {
+      AddContext(Declaration(name, inputTpe, outputTpe));
+    }
+    // In-place extension
+    method Extend(e: SExpr)
+      requires Valid()
+      modifies this, solver, solver.process
+      ensures Valid()
+      ensures assumptions == B.Cons(Assumption(e), old(assumptions))
+      ensures assumptionsStacks.head.Cons?
+      ensures assumptionsStacks == old(assumptionsStacks.(
+        head := B.Cons(Assumption(e), assumptionsStacks.head)))
+    {
+      AddContext(Assumption(e));
+    }
+
+    method Prove(e: SExpr) returns (result: ProofResult )
+      requires Valid()
+      ensures Valid()
+      modifies this, solver, solver.process
+      ensures assumptions == old(assumptions)
+    {
+      Push();
+      assert assumptionsSyncCommands(assumptionsStacks.tail, solver.CommandStacks().tail);
+      Extend(SExpr.Negation(e));
+      var satness := solver.CheckSat();
+      if satness == "unsat" {
+        result := Proved;
+      } else {
+        var model := solver.GetModel();
+        result := Unproved(satness + "\n" + model);
+      }
+      Pop();
+    }
+  }
 
   datatype Solver =
-    // TODO
-    Solver(assumptions: seq<SExpr>)
+    Solver(assumptions: seq<Context>)
   {
-    method Extend(e: SExpr) returns (solver: Solver) {
-      solver := Solver(assumptions + [e]);
+    static function Empty(): Solver {
+      Solver([])
     }
-    method Prove(e: SExpr) {
+    // Forking is costly as it creates a new SMT process
+    // and it will replay all assumptions till then
+    // but it is necessary if we plan on verifying in a previous solver state.
+    method Fork() returns (newSolverState: SolverState)
+      ensures fresh(newSolverState)
+      ensures newSolverState.ValidFor(this)
+    {
+      var newSolver := Z3SmtSolver.CreateZ3Solver();
+      newSolverState := new SolverState(newSolver);
+      assert newSolverState.ValidFor(Solver([]));
+      for i := 0 to |assumptions|
+        invariant newSolverState.ValidFor(Solver(assumptions[0..i]))
+        invariant newSolverState.Valid()
+      {
+        newSolverState.AddContext(assumptions[i]);
+      }
+      assert assumptions[0..|assumptions|] == assumptions;
+      assert newSolverState.ValidFor(this);
+    }
+    method Extend(e: SExpr, s: SolverState) returns (newSolver: Solver)
+      requires s.Valid()
+      requires s.ValidFor(this)
+      modifies s, s.solver, s.solver.process
+      ensures s.ValidFor(newSolver)
+      ensures s.Valid()
+    {
+      newSolver := Solver(assumptions + [Assumption(e)]);
+      s.Extend(e);
+    }
+    method Prove(e: SExpr, s: SolverState)
+      requires s.Valid() && s.ValidFor(this)
+      modifies s, s.solver, s.solver.process
+      ensures s.Valid() && s.ValidFor(this)
+    {
       // TODO
       print "----- Proof obligation:\n";
       for i := 0 to |assumptions| {
@@ -20,6 +222,8 @@ module Solvers {
       }
       print "  |-\n";
       print "  ", e, "\n";
+      var proofResult := s.Prove(e);
+      print "Result:", proofResult, "\n";
     }
     method Record(e: SExpr) returns (solver: Solver)
     { solver := this; } // TODO
